ulib/experimental/Steel.ST.ArraySlice.fst
@@ -1,0 +1,745 @@
+module Steel.ST.ArraySlice
+open Steel.ST.Util
+
+module A = Steel.ST.Array
+module R = Steel.ST.GhostPCMReference
+module P = Steel.PCMFrac
+module M = FStar.Map
+module PM = Steel.PCMMap
+module U32 = FStar.UInt32
+
+/// Gather permissions on reference [r]
+let derive_composable (#o:inames)
+           (#a:Type)
+           (#p:P.pcm a)
+           (r:R.ref a p)
+           (v0:a)
+           (v1:a)
+  : STGhost unit o
+           (R.pts_to r v0 `star` R.pts_to r v1)
+           (fun _ -> R.pts_to r v0 `star` R.pts_to r v1)
+           True
+           (fun _ -> FStar.PCM.composable p v0 v1)
+= R.gather r v0 v1;
+  R.share r _ v0 v1
+
+[@@noextract_to "krml"]
+let index_t (len: nat) : Tot eqtype = (i: nat { i < len })
+
+[@@noextract_to "krml"]
+let carrier (elt: Type u#a) (len: nat) : Tot Type =
+  PM.map (index_t len) (P.fractional elt)
+
+[@@noextract_to "krml"]
+let pcm (elt: Type u#a) (len: nat) : Tot (P.pcm (carrier elt len)) =
+  PM.pointwise (index_t len) (P.pcm_frac #elt)
+
+[@@noextract_to "krml"]
+let one (#elt: Type) (#len: nat) = (pcm elt len).P.p.P.one
+let composable (#elt: Type) (#len: nat) = (pcm elt len).P.p.P.composable
+[@@noextract_to "krml"]
+let compose (#elt: Type) (#len: nat) = (pcm elt len).P.p.P.op
+
+[@@noextract_to "krml"]
+let mk_carrier
+  (#elt: Type)
+  (len: nat)
+  (offset: nat)
+  (s: Seq.seq elt)
+  (p: P.perm)
+: Tot (carrier elt len)
+= let f (i: index_t len) : Tot (P.fractional elt) =
+    if offset + Seq.length s > len || i < offset || i >= offset + Seq.length s
+    then None
+    else Some (Seq.index s (i - offset), p)
+  in
+  M.map_literal f
+
+[@@__reduce__]
+let invariant0
+  (#elt: Type)
+  (base: A.array elt)
+  (gr: R.ref _ (pcm elt (A.length base)))
+: Tot vprop
+= exists_ (fun (whole_seq: Seq.seq elt) ->
+    A.pts_to base P.full_perm whole_seq `star`
+    R.pts_to gr (mk_carrier (A.length base) 0 whole_seq (P.half_perm P.full_perm)) `star`
+    pure (Seq.length whole_seq == A.length base)
+  )
+
+let invariant
+  (#elt: Type)
+  (base: A.array elt)
+  (gr: R.ref _ (pcm elt (A.length base)))
+: Tot vprop
+= invariant0 base gr
+
+noeq
+type array_slice (elt: Type) = {
+  base: A.array elt;
+  base_gr: R.ref _ (pcm elt (A.length base));
+  base_inv: inv (invariant base base_gr);
+  base_len: Ghost.erased U32.t; // to prove that A.read, A.write offset computation does not overflow
+  offset: U32.t;
+  length: Ghost.erased U32.t;
+  prf: squash (U32.v offset + U32.v length <= A.length base /\ U32.v base_len == A.length base);
+}
+
+let len (#elt: Type) (a: array_slice elt) : GTot U32.t =
+  a.length
+
+let length (#elt: Type) (a: array_slice elt) : GTot nat =
+  U32.v (len a)
+
+let valid_perm
+  (len: nat)
+  (offset: nat)
+  (slice_len: nat)
+  (p: P.perm) : Tot prop =
+  let open FStar.Real in
+  ((offset + slice_len <= len /\ slice_len > 0) ==> (p.P.v <=. one))
+
+[@@__reduce__]
+let pts_to0 (#elt: Type) (a: array_slice elt) (p: P.perm) (s: Seq.seq elt) : Tot vprop =
+  R.pts_to a.base_gr (mk_carrier (A.length a.base) (U32.v a.offset) s (P.half_perm p)) `star`
+  pure (
+    valid_perm (A.length a.base) (U32.v a.offset) (Seq.length s) (P.half_perm p) /\
+    Seq.length s == length a
+  )
+
+let pts_to (#elt: Type) (a: array_slice elt) ([@@@ smt_fallback ] p: P.perm) ([@@@ smt_fallback ] s: Seq.seq elt) : Tot vprop =
+  pts_to0 a p s
+
+let valid_sum_perm
+  (len: nat)
+  (offset: nat)
+  (slice_len: nat)
+  (p1 p2: perm)
+: Tot prop
+= let open FStar.Real in
+  valid_perm len offset slice_len (P.sum_perm p1 p2)
+
+let mk_carrier_valid_sum_perm
+  (#elt: Type)
+  (len: nat)
+  (offset: nat)
+  (s: Seq.seq elt)
+  (p1 p2: P.perm)
+: Lemma
+  (let c1 = mk_carrier len offset s p1 in
+   let c2 = mk_carrier len offset s p2 in
+   composable c1 c2 <==> valid_sum_perm len offset (Seq.length s) p1 p2)
+= let c1 = mk_carrier len offset s p1 in
+  let c2 = mk_carrier len offset s p2 in
+  if Seq.length s > 0 && offset + Seq.length s <= len
+  then
+    let open FStar.Real in
+    assert (P.composable (M.sel c1 offset) (M.sel c2 offset) <==> valid_perm len offset (Seq.length s) (P.sum_perm p1 p2))
+  else ()
+
+let mk_carrier_perm
+  (#elt: Type)
+  (len: nat)
+  (offset: nat)
+  (s: Seq.seq elt)
+  (p1 p2: P.perm)
+: Lemma
+  (requires (valid_sum_perm len offset (Seq.length s) p1 p2))
+  (ensures (
+    let c1 = mk_carrier len offset s p1 in
+    let c2 = mk_carrier len offset s p2 in
+      composable c1 c2 /\
+      mk_carrier len offset s (p1 `P.sum_perm` p2) `M.equal` (c1 `compose` c2)
+  ))
+= ()
+
+inline_for_extraction
+[@@noextract_to "krml"]
+let alloc
+  (#elt: Type)
+  (x: elt)
+  (n: U32.t)
+: ST (array_slice elt)
+    emp
+    (fun a -> pts_to a P.full_perm (Seq.create (U32.v n) x))
+    True
+    (fun a -> len a == n)
+=
+  let base = A.alloc x n in
+  let c = Ghost.hide (mk_carrier (A.length base) 0 (Seq.create (U32.v n) x) P.full_perm) in
+  let base_gr : R.ref _ (pcm elt (A.length base)) = R.alloc (Ghost.reveal c) in
+  mk_carrier_perm (A.length base) 0 (Seq.create (U32.v n) x) (P.half_perm P.full_perm) (P.half_perm P.full_perm);
+  let c_h = Ghost.hide (mk_carrier (A.length base) 0 (Seq.create (U32.v n) x) (P.half_perm P.full_perm)) in
+  R.share base_gr c c_h c_h;
+  rewrite
+    (invariant0 base base_gr)
+    (invariant base base_gr);
+  let i = new_invariant (invariant base base_gr) in
+  let a = {
+    base = base;
+    base_gr = base_gr;
+    base_len = Ghost.hide n;
+    base_inv = i;
+    offset = 0ul;
+    length = Ghost.hide n;
+    prf = ();
+  }
+  in
+  rewrite
+    (R.pts_to base_gr c_h)
+    (R.pts_to a.base_gr c_h);
+  rewrite
+    (pts_to0 a P.full_perm (Seq.create (U32.v n) x))
+    (pts_to a P.full_perm (Seq.create (U32.v n) x));
+  return a
+
+let share
+  (#opened: _)
+  (#elt: Type)
+  (#x: Seq.seq elt)
+  (a: array_slice elt)
+  (p p1 p2: P.perm)
+: STGhost unit opened
+    (pts_to a p x)
+    (fun _ -> pts_to a p1 x `star` pts_to a p2 x)
+    (p == p1 `P.sum_perm` p2)
+    (fun _ -> True)
+= rewrite
+    (pts_to a p x)
+    (pts_to0 a p x);
+  let _ = gen_elim () in
+  mk_carrier_perm (A.length a.base) (U32.v a.offset) x (P.half_perm p1) (P.half_perm p2);
+  R.share a.base_gr _
+    (mk_carrier (A.length a.base) (U32.v a.offset) x (P.half_perm p1))
+    (mk_carrier (A.length a.base) (U32.v a.offset) x (P.half_perm p2));
+  rewrite
+    (pts_to0 a p1 x)
+    (pts_to a p1 x);
+  rewrite
+    (pts_to0 a p2 x)
+    (pts_to a p2 x)
+
+let gather
+  (#opened: _)
+  (#elt: Type)
+  (#x: Seq.seq elt)
+  (a: array_slice elt)
+  (p1 p2: P.perm)
+: STGhostT unit opened
+    (pts_to a p1 x `star` pts_to a p2 x)
+    (fun _ -> pts_to a (p1 `P.sum_perm` p2) x)
+= rewrite
+    (pts_to a p1 x)
+    (pts_to0 a p1 x);
+  rewrite
+    (pts_to a p2 x)
+    (pts_to0 a p2 x);
+  let _ = gen_elim () in
+  derive_composable
+    a.base_gr
+    (mk_carrier (A.length a.base) (U32.v a.offset) x (P.half_perm p1))
+    (mk_carrier (A.length a.base) (U32.v a.offset) x (P.half_perm p2));
+  mk_carrier_valid_sum_perm (A.length a.base) (U32.v a.offset) x (P.half_perm p1) (P.half_perm p2);
+  mk_carrier_perm (A.length a.base) (U32.v a.offset) x (P.half_perm p1) (P.half_perm p2);
+  R.gather a.base_gr
+    (mk_carrier (A.length a.base) (U32.v a.offset) x (P.half_perm p1))
+    (mk_carrier (A.length a.base) (U32.v a.offset) x (P.half_perm p2));
+  rewrite
+    (pts_to0 a (p1 `P.sum_perm` p2) x)
+    (pts_to a (p1 `P.sum_perm` p2) x)
+
+let mk_carrier_index
+  (#elt: Type)
+  (len: nat)
+  (offset1: nat)
+  (s1: Seq.seq elt)
+  (p1: P.perm)
+  (offset2: nat)
+  (s2: Seq.seq elt)
+  (p2: P.perm)
+  (i1: nat)
+  (i2: nat)
+  (_: squash (
+    composable
+      (mk_carrier len offset1 s1 p1)
+      (mk_carrier len offset2 s2 p2) /\
+    offset1 + Seq.length s1 <= len /\
+    i1 < Seq.length s1 /\
+    offset2 + Seq.length s2 <= len /\
+    i2 < Seq.length s2 /\
+    offset1 + i1 == offset2 + i2
+  ))
+: Lemma
+  (ensures (
+    let o_l = mk_carrier len offset1 s1 p1 in
+    let o_r = mk_carrier len offset2 s2 p2 in
+    M.sel o_l (offset1 + i1) == Some (Seq.index s1 i1, p1) /\
+    M.sel o_r (offset2 + i2) == Some (Seq.index s2 i2, p2) /\
+    M.sel (compose o_l o_r) (offset1 + i1) == Some (Seq.index s1 i1, p1 `P.sum_perm` p2) /\
+    M.sel (compose o_l o_r) (offset2 + i2) == Some (Seq.index s2 i2, p1 `P.sum_perm` p2) /\
+    Seq.index s1 i1 == Seq.index s2 i2
+  ))
+= ()
+
+[@@noextract_to "krml"]
+let seq_index
+  (#t: Type)
+  (s: Seq.seq t)
+  (i: nat)
+: Pure t
+    (requires (i < Seq.length s))
+    (ensures (fun _ -> True))
+= Seq.index s i
+
+inline_for_extraction
+[@@noextract_to "krml"]
+let read_body
+  (#t: Type) (#p: perm) (#opened: _)
+  (a: array_slice t)
+  (#s: Ghost.erased (Seq.seq t))
+  (i: U32.t)
+  (_: unit)
+: STAtomicT t opened
+    (invariant a.base a.base_gr `star` (pts_to a p s `star` pure ((U32.v i < length a) == true)))
+    (fun res -> invariant a.base a.base_gr `star` (pts_to a p s `star` pure (U32.v i < Seq.length s /\ res == seq_index s (U32.v i))))
+=
+  rewrite
+    (invariant a.base a.base_gr)
+    (invariant0 a.base a.base_gr);
+  rewrite
+    (pts_to a p s)
+    (pts_to0 a p s);
+  let _ = gen_elim () in
+  derive_composable #_ #(carrier t (A.length a.base))
+    a.base_gr
+    (mk_carrier (A.length a.base) 0 _ (P.half_perm P.full_perm))
+    (mk_carrier (A.length a.base) (U32.v a.offset) s (P.half_perm p));
+  let full = vpattern_erased (fun full -> A.pts_to a.base P.full_perm full) in
+  mk_carrier_index (A.length a.base)
+    0 full (P.half_perm P.full_perm)
+    (U32.v a.offset) s (P.half_perm p)
+    (U32.v a.offset + U32.v i) (U32.v i) ();
+  let res = A.read a.base (a.offset `U32.add` i) in
+  rewrite
+    (invariant0 a.base a.base_gr)
+    (invariant a.base a.base_gr);
+  rewrite
+    (pts_to0 a p s)
+    (pts_to a p s);
+  return res
+
+inline_for_extraction
+[@@noextract_to "krml"]
+let atomic_read (#t:Type) (#p:perm) (#opened: _)
+         (a:array_slice t)
+         (#s:Ghost.erased (Seq.seq t))
+         (i:U32.t)
+: STAtomic t opened
+       (pts_to a p s)
+       (fun _ -> pts_to a p s)
+       (requires (
+         not (mem_inv opened a.base_inv) /\ // FIXME: HOW HOW HOW to prove this precondition if atomicity is needed?
+         U32.v i < length a
+       ))
+       (ensures fun v ->
+         U32.v i < Seq.length s /\
+         v == seq_index s (U32.v i))
+= noop ();
+  let res = with_invariant a.base_inv (read_body a i) in
+  let _ = gen_elim () in
+  return res
+
+inline_for_extraction
+[@@noextract_to "krml"]
+let read (#t:Type) (#p:perm)
+         (a:array_slice t)
+         (#s:Ghost.erased (Seq.seq t))
+         (i:U32.t)
+: ST t
+       (pts_to a p s)
+       (fun _ -> pts_to a p s)
+       (requires (
+         U32.v i < length a
+       ))
+       (ensures fun v ->
+         U32.v i < Seq.length s /\
+         v == seq_index s (U32.v i))
+= atomic_read a i
+
+let mk_carrier_upd
+  (#elt: Type)
+  (full: Seq.seq elt)
+  (offset: nat)
+  (s: Seq.seq elt)
+  (i: nat)
+  (v: elt)
+  (_: squash (
+    composable
+      (mk_carrier (Seq.length full) 0 full (P.half_perm P.full_perm))
+      (mk_carrier (Seq.length full) offset s (P.half_perm P.full_perm)) /\
+    offset + Seq.length s <= Seq.length full /\
+    i < Seq.length s
+  ))
+: Lemma
+  (ensures (
+    let o = compose
+      (mk_carrier (Seq.length full) 0 full (P.half_perm P.full_perm))
+      (mk_carrier (Seq.length full) offset s (P.half_perm P.full_perm))
+    in
+    let nl = mk_carrier (Seq.length full) 0 (Seq.upd full (offset + i) v) (P.half_perm P.full_perm) in
+    let nr = mk_carrier (Seq.length full) offset (Seq.upd s i v) (P.half_perm P.full_perm) in
+    composable nl nr /\
+    compose nl nr `Map.equal` Map.upd o (offset + i) (Some (v, P.full_perm))
+  ))
+= ()
+
+inline_for_extraction
+[@@noextract_to "krml"]
+let write_body
+  (#t: Type) (#opened: _)
+  (a: array_slice t)
+  (s: Ghost.erased (Seq.seq t))
+  (i: U32.t)
+  (sq: squash (U32.v i < Seq.length s))
+  (v: t)
+  (_: unit)
+: STAtomicT unit opened
+    (invariant a.base a.base_gr `star` pts_to a P.full_perm s)
+    (fun res -> invariant a.base a.base_gr `star` pts_to a P.full_perm (Seq.upd s (U32.v i) v))
+=
+  rewrite
+    (invariant a.base a.base_gr)
+    (invariant0 a.base a.base_gr);
+  rewrite
+    (pts_to a P.full_perm s)
+    (pts_to0 a P.full_perm s);
+  let _ = gen_elim () in
+  let o_r = Ghost.hide (mk_carrier (A.length a.base) (U32.v a.offset) s (P.half_perm P.full_perm)) in
+  let _ = R.gather #_ #(carrier t (A.length a.base))
+    a.base_gr _ (mk_carrier (A.length a.base) (U32.v a.offset) s (P.half_perm P.full_perm))
+  in
+  let full = vpattern_erased (fun full -> A.pts_to a.base P.full_perm full) in
+  let o_l = Ghost.hide (mk_carrier (A.length a.base) 0 full (P.half_perm P.full_perm)) in
+  let o = Ghost.hide (compose o_l o_r <: carrier t (A.length a.base)) in
+  mk_carrier_index (A.length a.base)
+    0 full (P.half_perm P.full_perm)
+    (U32.v a.offset) s (P.half_perm P.full_perm)
+    (U32.v a.offset + U32.v i) (U32.v i) ();
+  mk_carrier_upd full
+    (U32.v a.offset) s
+    (U32.v i) v ();
+  A.write a.base (a.offset `U32.add` i) v;
+  R.upd_gen
+    a.base_gr
+    _ _
+    (PM.lift_frame_preserving_upd
+      _ _
+      (P.mk_frame_preserving_upd
+        (Seq.index s (U32.v i))
+        v
+      )
+      o (U32.v a.offset + U32.v i)
+    );
+  R.share
+    a.base_gr
+    _
+    (mk_carrier (A.length a.base) 0 (Seq.upd full (U32.v a.offset + U32.v i) v) (P.half_perm P.full_perm))
+    (mk_carrier (A.length a.base) (U32.v a.offset) (Seq.upd s (U32.v i) v) (P.half_perm P.full_perm));
+  rewrite
+    (pts_to0 a P.full_perm (Seq.upd s (U32.v i) v))
+    (pts_to a P.full_perm (Seq.upd s (U32.v i) v));
+  assert_ (A.pts_to a.base P.full_perm (Seq.upd full (U32.v a.offset + U32.v i) v)); // FIXME: WHY WHY WHY?
+  rewrite
+    (invariant0 a.base a.base_gr)
+    (invariant a.base a.base_gr)
+
+inline_for_extraction
+[@@noextract_to "krml"]
+let atomic_write (#t:Type) (#opened: _)
+         (a:array_slice t)
+         (#s:Ghost.erased (Seq.seq t))
+         (i:U32.t)
+         (v: t)
+: STAtomic (Ghost.erased (Seq.seq t)) opened
+       (pts_to a P.full_perm s)
+       (fun s' -> pts_to a P.full_perm s')
+       (requires (
+         not (mem_inv opened a.base_inv) /\ // FIXME: HOW HOW HOW to prove this precondition if atomicity is needed?
+         U32.v i < length a
+       ))
+       (ensures fun s' ->
+         U32.v i < Seq.length s /\
+         Ghost.reveal s' == Seq.upd s (U32.v i) v)
+= rewrite
+    (pts_to a P.full_perm s)
+    (pts_to0 a P.full_perm s);
+  let _ = gen_elim () in
+  rewrite
+    (pts_to0 a P.full_perm s)
+    (pts_to a P.full_perm s);
+  with_invariant a.base_inv (write_body a s i () v);
+  let _ = gen_elim () in
+  vpattern_replace_erased (fun s' -> pts_to a P.full_perm s')
+
+inline_for_extraction
+[@@noextract_to "krml"]
+let write (#t:Type)
+         (a:array_slice t)
+         (#s:Ghost.erased (Seq.seq t))
+         (i:U32.t)
+         (v: t)
+: ST (Ghost.erased (Seq.seq t))
+       (pts_to a P.full_perm s)
+       (fun s' -> pts_to a P.full_perm s')
+       (requires (
+         U32.v i < length a
+       ))
+       (ensures fun s' ->
+         U32.v i < Seq.length s /\
+         Ghost.reveal s' == Seq.upd s (U32.v i) v)
+= atomic_write a i v
+
+let adjacent (#elt: Type) (a1 a2: array_slice elt) : Tot prop =
+  a1.base == a2.base /\
+  a1.base_gr == a2.base_gr /\
+  a1.base_inv == a2.base_inv /\
+  U32.v a1.offset + U32.v a1.length == U32.v a2.offset
+
+inline_for_extraction
+[@@noextract_to "krml"]
+let merge (#elt: Type) (a1 a2: array_slice elt)
+: Pure (array_slice elt)
+  (requires (adjacent a1 a2))
+  (ensures (fun y -> length y == length a1 + length a2))
+= {
+  base = a1.base;
+  base_gr = a1.base_gr;
+  base_inv = a1.base_inv;
+  base_len = a1.base_len;
+  offset = a1.offset;
+  length = U32.add a1.length a2.length;
+  prf = ();
+}
+
+let merge_assoc (#elt: Type) (a1 a2 a3: array_slice elt) : Lemma
+  (requires (adjacent a1 a2 /\ adjacent a2 a3))
+  (ensures (
+    adjacent (merge a1 a2) a3 /\ adjacent a1 (merge a2 a3) /\
+    merge (merge a1 a2) a3 == merge a1 (merge a2 a3)
+  ))
+= ()
+
+let merge_into (#elt: Type) (a1 a2 a: array_slice elt) : Tot prop =
+  adjacent a1 a2 /\
+  merge a1 a2 == a
+
+let mk_carrier_merge
+  (#elt: Type)
+  (len: nat)
+  (offset: nat)
+  (s1 s2: Seq.seq elt)
+  (p: P.perm)
+: Lemma
+  (requires (
+    offset + Seq.length s1 + Seq.length s2 <= len
+  ))
+  (ensures (
+    let c1 = mk_carrier len offset s1 p in
+    let c2 = mk_carrier len (offset + Seq.length s1) s2 p in
+      composable c1 c2 /\
+      mk_carrier len offset (s1 `Seq.append` s2) p `M.equal` (c1 `compose` c2)
+  ))
+= ()
+
+let ghost_join
+  (#opened: _)
+  (#elt: Type)
+  (#x1 #x2: Seq.seq elt)
+  (#p: perm)
+  (a1 a2: array_slice elt)
+: STGhost (Ghost.erased (array_slice elt)) opened
+    (pts_to a1 p x1 `star` pts_to a2 p x2)
+    (fun res -> pts_to res p (x1 `Seq.append` x2))
+    (adjacent a1 a2)
+    (fun res -> merge_into a1 a2 res)
+= rewrite
+    (pts_to a1 p x1)
+    (pts_to0 a1 p x1);
+  rewrite
+    (pts_to a2 p x2)
+    (pts_to0 a2 p x2);
+  let _ = gen_elim () in
+  mk_carrier_merge (A.length a1.base) (U32.v a1.offset) x1 x2 (P.half_perm p);
+  rewrite
+    (R.pts_to a2.base_gr (mk_carrier (A.length a2.base) (U32.v a2.offset) x2 (P.half_perm p)))
+    (R.pts_to a1.base_gr (mk_carrier (A.length a1.base) (U32.v a1.offset + Seq.length x1) x2 (P.half_perm p)));
+  R.gather a1.base_gr
+    (mk_carrier (A.length a1.base) (U32.v a1.offset) x1 (P.half_perm p))
+    (mk_carrier (A.length a1.base) (U32.v a1.offset + Seq.length x1) x2 (P.half_perm p));
+  let res = Ghost.hide (merge a1 a2) in
+  rewrite
+    (R.pts_to a1.base_gr _)
+    (R.pts_to res.base_gr (mk_carrier (A.length res.base) (U32.v res.offset) (x1 `Seq.append` x2) (P.half_perm p)));
+  rewrite
+    (pts_to0 res p (Seq.append x1 x2))
+    (pts_to res p (Seq.append x1 x2));
+  res
+
+inline_for_extraction
+[@@noextract_to "krml"]
+let join
+  (#opened: _)
+  (#elt: Type)
+  (#x1 #x2: Ghost.erased (Seq.seq elt))
+  (#p: perm)
+  (a1 a2: array_slice elt)
+: STAtomicBase (array_slice elt) false opened Unobservable
+    (pts_to a1 p x1 `star` pts_to a2 p x2)
+    (fun res -> pts_to res p (x1 `Seq.append` x2))
+    (adjacent a1 a2)
+    (fun res -> merge_into a1 a2 res)
+= let g = ghost_join a1 a2 in
+  let res = merge a1 a2 in
+  rewrite
+    (pts_to g p (x1 `Seq.append` x2))
+    (pts_to res p (x1 `Seq.append` x2));
+  return res
+
+let mk_carrier_split
+  (#elt: Type)
+  (len: nat)
+  (offset: nat)
+  (s: Seq.seq elt)
+  (p: P.perm)
+  (i: nat)
+: Lemma
+  (requires (
+    offset + Seq.length s <= len /\
+    i <= Seq.length s
+  ))
+  (ensures (
+    let c1 = mk_carrier len offset (Seq.slice s 0 i) p in
+    let c2 = mk_carrier len (offset + i) (Seq.slice s i (Seq.length s)) p in
+      composable c1 c2 /\
+      mk_carrier len offset s p `M.equal` (c1 `compose` c2)
+  ))
+= ()
+
+inline_for_extraction
+[@@noextract_to "krml"]
+let tsplit (#elt: Type) (a: array_slice elt)
+  (i: U32.t)
+: Pure (array_slice elt & array_slice elt)
+  (requires (U32.v i <= length a))
+  (ensures (fun y -> merge_into (fst y) (snd y) a))
+= (
+    {
+      base = a.base;
+      base_gr = a.base_gr;
+      base_inv = a.base_inv;
+      base_len = a.base_len;
+      offset = a.offset;
+      length = i;
+      prf = ();
+    }, {
+      base = a.base;
+      base_gr = a.base_gr;
+      base_inv = a.base_inv;
+      base_len = a.base_len;
+      offset = a.offset `U32.add` i;
+      length = a.length `U32.sub` i;
+      prf = ();
+    }
+  )
+    
+#set-options "--ide_id_info_off"
+
+let ghost_split
+  (#opened: _)
+  (#elt: Type)
+  (#x: Seq.seq elt)
+  (#p: perm)
+  (a: array_slice elt)
+  (i: U32.t)
+: STGhost (Ghost.erased (array_slice elt & array_slice elt)) opened
+    (pts_to a p x)
+    (fun res -> exists_ (fun x1 -> exists_ (fun x2 ->
+      pts_to (fst res) p x1 `star`
+      pts_to (snd res) p x2 `star`
+      pure (
+        U32.v i <= length a /\
+        U32.v i <= Seq.length x /\
+        x1 == Seq.slice x 0 (U32.v i) /\
+        x2 == Seq.slice x (U32.v i) (Seq.length x) /\
+        x == x1 `Seq.append` x2 /\
+        Ghost.reveal res == tsplit a i
+    ))))
+    (U32.v i <= length a)
+    (fun _ -> True)
+= rewrite
+    (pts_to a p x)
+    (pts_to0 a p x);
+  let _ = gen_elim () in
+  mk_carrier_split
+    (A.length a.base)
+    (U32.v a.offset)
+    x
+    (P.half_perm p)
+    (U32.v i);
+  Seq.lemma_split x (U32.v i);
+  let xl = Seq.slice x 0 (U32.v i) in
+  let xr = Seq.slice x (U32.v i) (Seq.length x) in
+  let vl = mk_carrier (A.length a.base) (U32.v a.offset) xl (P.half_perm p) in
+  let vr = mk_carrier (A.length a.base) (U32.v a.offset + U32.v i) xr (P.half_perm p) in
+  R.share a.base_gr _ vl vr;
+  let res = Ghost.hide (tsplit a i) in
+  rewrite
+    (R.pts_to a.base_gr vl)
+    (R.pts_to (fst res).base_gr (mk_carrier (A.length (fst res).base) (U32.v (fst res).offset) xl (P.half_perm p)));
+  rewrite
+    (pts_to0 (fst res) p xl)
+    (pts_to (fst res) p xl);
+  rewrite
+    (R.pts_to a.base_gr vr)
+    (R.pts_to (snd res).base_gr (mk_carrier (A.length (snd res).base) (U32.v (snd res).offset) xr (P.half_perm p)));
+  rewrite
+    (pts_to0 (snd res) p xr)
+    (pts_to (snd res) p xr);
+  res
+
+inline_for_extraction
+[@@noextract_to "krml"]
+let split
+  (#opened: _)
+  (#elt: Type)
+  (#x: Ghost.erased (Seq.seq elt))
+  (#p: perm)
+  (a: array_slice elt)
+  (i: U32.t)
+: STAtomicBase (array_slice elt & array_slice elt) false opened Unobservable
+    (pts_to a p x)
+    (fun res -> exists_ (fun x1 -> exists_ (fun x2 ->
+      pts_to (fst res) p x1 `star`
+      pts_to (snd res) p x2 `star`
+      pure (
+        U32.v i <= length a /\
+        U32.v i <= Seq.length x /\
+        x1 == Seq.slice x 0 (U32.v i) /\
+        x2 == Seq.slice x (U32.v i) (Seq.length x) /\
+        Ghost.reveal x == x1 `Seq.append` x2 /\
+        res == tsplit a i
+    ))))
+    (U32.v i <= length a)
+    (fun _ -> True)
+= let g = ghost_split a i in
+  let _ = gen_elim () in
+  let res = tsplit a i in
+  let x1 = vpattern_erased (fun x1 -> pts_to (fst g) p x1) in
+  rewrite
+    (pts_to (fst g) p _)
+    (pts_to (fst res) p x1);
+  let x2 = vpattern_erased (fun x2 -> pts_to (snd g) p x2) in
+  rewrite
+    (pts_to (snd g) p _)
+    (pts_to (snd res) p x2);
+  return res
